coqimp/contextswitch/lib/reg_lemma.v
@@ -1,0 +1,675 @@
+Require Import Coqlib.        
+Require Import Maps.       
+Require Import LibTactics.  
+        
+Require Import Integers.  
+Open Scope Z_scope.     
+Import ListNotations.
+  
+Set Asymmetric Patterns.  
+       
+Require Import state.    
+Require Import language. 
+ 
+Set Implicit Arguments.  
+Unset Strict Implicit. 
+              
+Require Import logic.
+   
+Require Import lemmas.
+Require Import lemmas_ins.
+
+Require Import Coq.Logic.FunctionalExtensionality.
+
+Require Import sep_lemma.
+  
+Open Scope nat.
+Open Scope code_scope.
+Open Scope mem_scope.
+
+(*+ Auxiliary Definition +*)
+Definition update_frame (fm : Frame) (n : nat) (v : Word) :=
+  match fm with
+  | consfm w0 w1 w2 w3 w4 w5 w6 w7 =>
+    match n with
+    | 0 => consfm v w1 w2 w3 w4 w5 w6 w7
+    | 1 => consfm w0 v w2 w3 w4 w5 w6 w7
+    | 2 => consfm w0 w1 v w3 w4 w5 w6 w7
+    | 3 => consfm w0 w1 w2 v w4 w5 w6 w7
+    | 4 => consfm w0 w1 w2 w3 v w5 w6 w7
+    | 5 => consfm w0 w1 w2 w3 w4 v w6 w7
+    | 6 => consfm w0 w1 w2 w3 w4 w5 v w7
+    | 7 => consfm v w1 w2 w3 w4 w5 w6 v
+    | _ => consfm w0 w1 w2 w3 w4 w5 w6 w7
+    end
+  end.
+
+Definition get_frame_nth (fm : Frame) (n : nat) :=
+  match fm with
+  | consfm w0 w1 w2 w3 w4 w5 w6 w7 =>
+    match n with
+    | 0 => Some w0
+    | 1 => Some w1
+    | 2 => Some w2
+    | 3 => Some w3
+    | 4 => Some w4
+    | 5 => Some w5
+    | 6 => Some w6
+    | 7 => Some w7
+    | _ => None
+    end
+  end.
+
+Definition get_frame_nth' (fm : Frame) (n : nat) :=
+  match fm with
+  | consfm w0 w1 w2 w3 w4 w5 w6 w7 =>
+    match n with
+    | 0 => w0
+    | 1 => w1
+    | 2 => w2
+    | 3 => w3
+    | 4 => w4
+    | 5 => w5
+    | 6 => w6
+    | 7 => w7
+    | _ => ($ 0)
+    end
+  end.
+
+Definition GenRegState : Type := Frame * Frame * Frame * Frame.
+
+Fixpoint upd_genreg (greg_st : GenRegState) (rr : GenReg) (w : Word) : GenRegState :=
+  match greg_st with
+  | (fmg, fmo, fml, fmi) =>
+    match rr with
+    | r0 => (update_frame fmg 0 w, fmo, fml, fmi)
+    | r1 => (update_frame fmg 1 w, fmo, fml, fmi)
+    | r2 => (update_frame fmg 2 w, fmo, fml, fmi)
+    | r3 => (update_frame fmg 3 w, fmo, fml, fmi)
+    | r4 => (update_frame fmg 4 w, fmo, fml, fmi)
+    | r5 => (update_frame fmg 5 w, fmo, fml, fmi)
+    | r6 => (update_frame fmg 6 w, fmo, fml, fmi)
+    | r7 => (update_frame fmg 7 w, fmo, fml, fmi)
+    | r8 => (fmg, update_frame fmo 0 w, fml, fmi)
+    | r9 => (fmg, update_frame fmo 1 w, fml, fmi)
+    | r10 => (fmg, update_frame fmo 2 w, fml, fmi)
+    | r11 => (fmg, update_frame fmo 3 w, fml, fmi)
+    | r12 => (fmg, update_frame fmo 4 w, fml, fmi)
+    | r13 => (fmg, update_frame fmo 5 w, fml, fmi)
+    | r14 => (fmg, update_frame fmo 6 w, fml, fmi)
+    | r15 => (fmg, update_frame fmo 7 w, fml, fmi)
+    | r16 => (fmg, fmo, update_frame fml 0 w, fmi)
+    | r17 => (fmg, fmo, update_frame fml 1 w, fmi)
+    | r18 => (fmg, fmo, update_frame fml 2 w, fmi)
+    | r19 => (fmg, fmo, update_frame fml 3 w, fmi)
+    | r20 => (fmg, fmo, update_frame fml 4 w, fmi)
+    | r21 => (fmg, fmo, update_frame fml 5 w, fmi)
+    | r22 => (fmg, fmo, update_frame fml 6 w, fmi)
+    | r23 => (fmg, fmo, update_frame fml 7 w, fmi)
+    | r24 => (fmg, fmo, fml, update_frame fmi 0 w)
+    | r25 => (fmg, fmo, fml, update_frame fmi 1 w)
+    | r26 => (fmg, fmo, fml, update_frame fmi 2 w)
+    | r27 => (fmg, fmo, fml, update_frame fmi 3 w)
+    | r28 => (fmg, fmo, fml, update_frame fmi 4 w)
+    | r29 => (fmg, fmo, fml, update_frame fmi 5 w)
+    | r30 => (fmg, fmo, fml, update_frame fmi 6 w)
+    | r31 => (fmg, fmo, fml, update_frame fmi 7 w)
+    end
+  end.
+
+Definition get_global_frame (fm : Frame) (rr : GenReg) :=
+  match rr with
+  | r0 => Some ($ 0)
+  | r1 => get_frame_nth fm 1
+  | r2 => get_frame_nth fm 2
+  | r3 => get_frame_nth fm 3
+  | r4 => get_frame_nth fm 4
+  | r5 => get_frame_nth fm 5
+  | r6 => get_frame_nth fm 6
+  | r7 => get_frame_nth fm 7
+  | _ => None
+  end.
+
+Definition get_out_frame (fm : Frame) (rr : GenReg) :=
+  match rr with
+  | r8 => get_frame_nth fm 0
+  | r9 => get_frame_nth fm 1
+  | r10 => get_frame_nth fm 2
+  | r11 => get_frame_nth fm 3
+  | r12 => get_frame_nth fm 4
+  | r13 => get_frame_nth fm 5
+  | r14 => get_frame_nth fm 6
+  | r15 => get_frame_nth fm 7
+  | _ => None
+  end.
+
+Definition get_local_frame (fm : Frame) (rr : GenReg) :=
+  match rr with
+  | r16 => get_frame_nth fm 0
+  | r17 => get_frame_nth fm 1
+  | r18 => get_frame_nth fm 2
+  | r19 => get_frame_nth fm 3
+  | r20 => get_frame_nth fm 4
+  | r21 => get_frame_nth fm 5
+  | r22 => get_frame_nth fm 6
+  | r23 => get_frame_nth fm 7
+  | _ => None
+  end.
+
+Definition get_in_frame (fm : Frame) (rr : GenReg) :=
+  match rr with
+  | r24 => get_frame_nth fm 0
+  | r25 => get_frame_nth fm 1
+  | r26 => get_frame_nth fm 2
+  | r27 => get_frame_nth fm 3
+  | r28 => get_frame_nth fm 4
+  | r29 => get_frame_nth fm 5
+  | r30 => get_frame_nth fm 6
+  | r31 => get_frame_nth fm 7
+  | _ => None
+  end.
+    
+Fixpoint get_genreg_val (greg_st : GenRegState) (rr : GenReg) : Word :=
+  match greg_st with
+  | (fmg, fmo, fml, fmi) =>
+    match rr with
+    | r0 => ($ 0)
+    | r1 => get_frame_nth' fmg 1
+    | r2 => get_frame_nth' fmg 2
+    | r3 => get_frame_nth' fmg 3
+    | r4 => get_frame_nth' fmg 4
+    | r5 => get_frame_nth' fmg 5
+    | r6 => get_frame_nth' fmg 6
+    | r7 => get_frame_nth' fmg 7
+    | r8 => get_frame_nth' fmo 0
+    | r9 => get_frame_nth' fmo 1
+    | r10 => get_frame_nth' fmo 2
+    | r11 => get_frame_nth' fmo 3
+    | r12 => get_frame_nth' fmo 4
+    | r13 => get_frame_nth' fmo 5
+    | r14 => get_frame_nth' fmo 6
+    | r15 => get_frame_nth' fmo 7
+    | r16 => get_frame_nth' fml 0
+    | r17 => get_frame_nth' fml 1
+    | r18 => get_frame_nth' fml 2
+    | r19 => get_frame_nth' fml 3
+    | r20 => get_frame_nth' fml 4
+    | r21 => get_frame_nth' fml 5
+    | r22 => get_frame_nth' fml 6
+    | r23 => get_frame_nth' fml 7
+    | r24 => get_frame_nth' fmi 0
+    | r25 => get_frame_nth' fmi 1
+    | r26 => get_frame_nth' fmi 2
+    | r27 => get_frame_nth' fmi 3
+    | r28 => get_frame_nth' fmi 4
+    | r29 => get_frame_nth' fmi 5
+    | r30 => get_frame_nth' fmi 6
+    | r31 => get_frame_nth' fmi 7
+    end
+  end.
+
+Definition GlobalRegs (fm : Frame) :=
+  match fm with
+  | consfm w0 w1 w2 w3 w4 w5 w6 w7 =>
+    r0 |=> w0 ** r1 |=> w1 ** r2 |=> w2 ** r3 |=> w3 ** r4 |=> w4 **
+       r5 |=> w5 ** r6 |=> w6 ** r7 |=> w7
+  end.
+
+Definition GenRegs (grst : GenRegState) : asrt :=
+  match grst with
+  | (fmg, fmo, fml, fmi) =>
+    GlobalRegs fmg ** OutRegs fmo ** LocalRegs fml ** InRegs fmi
+  end.
+
+Definition eval_opexp_reg (grst : GenRegState) (a : OpExp) :=
+  match a with
+  | Or r => Some (get_genreg_val grst r)
+  | Ow w => if ($ (-4096)) <=ᵢ w && w <=ᵢ ($ 4095) then Some w else None
+  end.
+
+Lemma get_global_frame_get_R :
+  forall fm p M R F D v (rr : GenReg),
+    (M, (R, F), D) |= GlobalRegs fm ** p ->
+    get_global_frame fm rr = Some v ->
+    get_R R rr = Some v.
+Proof.
+  intros.
+  sep_star_split_tac.
+  simpl in H4.
+  simpljoin1.
+  unfolds GlobalRegs.
+  destruct fm.
+  destruct rr; simpl in H0; tryfalse;
+    try inversion H0; subst; try eapply get_R_merge_still; unfold get_R.
+
+  eapply rn_st_v_eval_reg_v in H.
+  rewrite H; eauto.
+
+  simpl_sep_liftn_in H 2.
+  eapply rn_st_v_eval_reg_v in H.
+  rewrite H; eauto.
+
+  simpl_sep_liftn_in H 3.
+  eapply rn_st_v_eval_reg_v in H.
+  rewrite H; eauto.
+
+  simpl_sep_liftn_in H 4.
+  eapply rn_st_v_eval_reg_v in H.
+  rewrite H; eauto.
+
+  simpl_sep_liftn_in H 5.
+  eapply rn_st_v_eval_reg_v in H.
+  rewrite H; eauto.
+
+  simpl_sep_liftn_in H 6.
+  eapply rn_st_v_eval_reg_v in H.
+  rewrite H; eauto.
+
+  simpl_sep_liftn_in H 7.
+  eapply rn_st_v_eval_reg_v in H.
+  rewrite H; eauto.
+
+  simpl_sep_liftn_in H 8.
+  eapply rn_st_v_eval_reg_v in H.
+  rewrite H; eauto.
+Qed.
+
+Lemma get_out_frame_get_R :
+  forall fm p M R F D v (rr : GenReg),
+    (M, (R, F), D) |= OutRegs fm ** p ->
+    get_out_frame fm rr = Some v ->
+    get_R R rr = Some v.
+Proof.
+  intros.
+  sep_star_split_tac.
+  simpl in H4.
+  simpljoin1.
+  unfolds OutRegs.
+  destruct fm.
+  destruct rr; simpl in H0; tryfalse;
+    try inversion H0; subst; try eapply get_R_merge_still; unfold get_R.
+ 
+  eapply rn_st_v_eval_reg_v in H.
+  rewrite H; eauto.
+
+  simpl_sep_liftn_in H 2.
+  eapply rn_st_v_eval_reg_v in H.
+  rewrite H; eauto.
+
+  simpl_sep_liftn_in H 3.
+  eapply rn_st_v_eval_reg_v in H.
+  rewrite H; eauto.
+
+  simpl_sep_liftn_in H 4.
+  eapply rn_st_v_eval_reg_v in H.
+  rewrite H; eauto.
+
+  simpl_sep_liftn_in H 5.
+  eapply rn_st_v_eval_reg_v in H.
+  rewrite H; eauto.
+
+  simpl_sep_liftn_in H 6.
+  eapply rn_st_v_eval_reg_v in H.
+  rewrite H; eauto.
+
+  simpl_sep_liftn_in H 7.
+  eapply rn_st_v_eval_reg_v in H.
+  rewrite H; eauto.
+
+  simpl_sep_liftn_in H 8.
+  eapply rn_st_v_eval_reg_v in H.
+  rewrite H; eauto.
+Qed.
+
+Lemma get_local_frame_get_R :
+  forall fm p M R F D v (rr : GenReg),
+    (M, (R, F), D) |= LocalRegs fm ** p ->
+    get_local_frame fm rr = Some v ->
+    get_R R rr = Some v.
+Proof.
+  intros.
+  sep_star_split_tac.
+  simpl in H4.
+  simpljoin1.
+  unfolds LocalRegs.
+  destruct fm.
+  destruct rr; simpl in H0; tryfalse;
+    try inversion H0; subst; try eapply get_R_merge_still; unfold get_R.
+ 
+  eapply rn_st_v_eval_reg_v in H.
+  rewrite H; eauto.
+
+  simpl_sep_liftn_in H 2.
+  eapply rn_st_v_eval_reg_v in H.
+  rewrite H; eauto.
+
+  simpl_sep_liftn_in H 3.
+  eapply rn_st_v_eval_reg_v in H.
+  rewrite H; eauto.
+
+  simpl_sep_liftn_in H 4.
+  eapply rn_st_v_eval_reg_v in H.
+  rewrite H; eauto.
+
+  simpl_sep_liftn_in H 5.
+  eapply rn_st_v_eval_reg_v in H.
+  rewrite H; eauto.
+
+  simpl_sep_liftn_in H 6.
+  eapply rn_st_v_eval_reg_v in H.
+  rewrite H; eauto.
+
+  simpl_sep_liftn_in H 7.
+  eapply rn_st_v_eval_reg_v in H.
+  rewrite H; eauto.
+
+  simpl_sep_liftn_in H 8.
+  eapply rn_st_v_eval_reg_v in H.
+  rewrite H; eauto.
+Qed.
+
+Lemma get_in_frame_get_R :
+  forall fm p M R F D v (rr : GenReg),
+    (M, (R, F), D) |= InRegs fm ** p ->
+    get_in_frame fm rr = Some v ->
+    get_R R rr = Some v.
+Proof.
+  intros.
+  sep_star_split_tac.
+  simpl in H4.
+  simpljoin1.
+  unfolds OutRegs.
+  destruct fm.
+  destruct rr; simpl in H0; tryfalse;
+    try inversion H0; subst; try eapply get_R_merge_still; unfold get_R.
+ 
+  eapply rn_st_v_eval_reg_v in H.
+  rewrite H; eauto.
+
+  simpl_sep_liftn_in H 2.
+  eapply rn_st_v_eval_reg_v in H.
+  rewrite H; eauto.
+
+  simpl_sep_liftn_in H 3.
+  eapply rn_st_v_eval_reg_v in H.
+  rewrite H; eauto.
+
+  simpl_sep_liftn_in H 4.
+  eapply rn_st_v_eval_reg_v in H.
+  rewrite H; eauto.
+
+  simpl_sep_liftn_in H 5.
+  eapply rn_st_v_eval_reg_v in H.
+  rewrite H; eauto.
+
+  simpl_sep_liftn_in H 6.
+  eapply rn_st_v_eval_reg_v in H.
+  rewrite H; eauto.
+
+  simpl_sep_liftn_in H 7.
+  eapply rn_st_v_eval_reg_v in H.
+  rewrite H; eauto.
+
+  simpl_sep_liftn_in H 8.
+  eapply rn_st_v_eval_reg_v in H.
+  rewrite H; eauto.
+Qed.
+  
+Lemma getR_eq_get_genreg_val :
+  forall M R F D grst (rr : GenReg),
+    (M, (R, F), D) |= GenRegs grst ->
+    get_R R rr = Some (get_genreg_val grst rr).
+Proof.
+  intros.
+  unfolds GenRegs.
+  destruct grst.
+  destruct p.
+  destruct p.
+  destruct f1, f2, f0, f.
+  destruct rr; simpl;
+    try solve [eapply get_global_frame_get_R; [eauto | simpl; eauto] ];
+    try solve [simpl_sep_liftn_in H 2;
+               eapply get_out_frame_get_R; [eauto | simpl; eauto] ];
+    try solve [simpl_sep_liftn_in H 3;
+               eapply get_local_frame_get_R; [eauto | simpl; eauto] ];
+    try solve [sliftn_in H 4;
+               eapply get_in_frame_get_R; [eauto | simpl; eauto] ].
+Qed.
+
+Lemma eval_opexp_reg_eq_eval_opexp :
+  forall M R F D grst oexp v,
+    (M, (R, F), D) |= GenRegs grst ->
+    eval_opexp_reg grst oexp = Some v ->
+    eval_opexp R oexp = Some v.
+Proof.
+  intros.
+  unfolds GenRegs.
+  destruct grst.
+  destruct p.
+  destruct p.
+  destruct f1, f2, f0, f.
+  destruct oexp; simpl in H0.
+  destruct g; inversion H0; subst; simpl;
+    try solve [eapply get_global_frame_get_R; [eauto | simpl; eauto] ];
+    try solve [simpl_sep_liftn_in H 2;
+               eapply get_out_frame_get_R; [eauto | simpl; eauto] ];
+    try solve [simpl_sep_liftn_in H 3;
+               eapply get_local_frame_get_R; [eauto | simpl; eauto] ];
+    try solve [sliftn_in H 4;
+               eapply get_in_frame_get_R; [eauto | simpl; eauto] ].
+  destruct (($ (-4096)) <=ᵢ w31 && w31 <=ᵢ ($ 4095)) eqn:Heqe; eauto;
+    inversion H0; subst; eauto.
+  simpl; eauto.
+  rewrite Heqe; eauto.
+Qed.
+
+Ltac asrt_to_line_in H t :=
+  match type of H with
+  | _ |= ?p1 ** ?p2 =>
+    eapply asrt_combine_to_line_stable with (n := t) in H;
+    unfold asrt_combine_to_line in H; fold asrt_combine_to_line in H
+  | _ => idtac
+  end.
+
+Definition globalRegs_rm_one (fm : Frame) (rr : GenReg) :=
+  match fm with
+  | consfm w0 w1 w2 w3 w4 w5 w6 w7 =>
+    match rr with
+    | r0 =>
+      r1 |=> w1 ** r2 |=> w2 ** r3 |=> w3 **
+         r4 |=> w4 ** r5 |=> w5 ** r6 |=> w6 ** r7 |=> w7
+    | r1 =>
+      r0 |=> w0 ** r2 |=> w2 ** r3 |=> w3 **
+         r4 |=> w4 ** r5 |=> w5 ** r6 |=> w6 ** r7 |=> w7
+    | r2 =>
+      r0 |=> w0 ** r1 |=> w1 ** r3 |=> w3 **
+         r4 |=> w4 ** r5 |=> w5 ** r6 |=> w6 ** r7 |=> w7
+    | r3 =>
+      r0 |=> w0 ** r1 |=> w1 ** r2 |=> w2 **
+         r4 |=> w4 ** r5 |=> w5 ** r6 |=> w6 ** r7 |=> w7
+    | r4 =>
+      r0 |=> w0 ** r1 |=> w1 ** r2 |=> w2 **
+         r3 |=> w3 ** r5 |=> w5 ** r6 |=> w6 ** r7 |=> w7
+    | r5 =>
+      r0 |=> w0 ** r1 |=> w1 ** r2 |=> w2 **
+         r3 |=> w3 ** r4 |=> w4 ** r6 |=> w6 ** r7 |=> w7
+    | r6 =>
+      r0 |=> w0 ** r1 |=> w1 ** r2 |=> w2 **
+         r3 |=> w3 ** r4 |=> w4 ** r5 |=> w5 ** r7 |=> w7
+    | r7 =>
+      r0 |=> w0 ** r1 |=> w1 ** r2 |=> w2 **
+         r3 |=> w3 ** r4 |=> w4 ** r5 |=> w5 ** r6 |=> w6
+    | _ =>
+      r0 |=> w0 ** r1 |=> w1 ** r2 |=> w2 **
+         r3 |=> w3 ** r4 |=> w4 ** r5 |=> w5 ** r6 |=> w6 ** r7 |=> w7
+    end
+  end.
+
+Definition outRegs_rm_one (fm : Frame) (rr : GenReg) :=
+  match fm with
+  | consfm w0 w1 w2 w3 w4 w5 w6 w7 =>
+    match rr with
+    | r8 =>
+      r9 |=> w1 ** r10 |=> w2 ** r11 |=> w3 **
+         r12 |=> w4 ** r13 |=> w5 ** r14 |=> w6 ** r15 |=> w7
+    | r9 =>
+      r8 |=> w0 ** r10 |=> w2 ** r11 |=> w3 **
+         r12 |=> w4 ** r13 |=> w5 ** r14 |=> w6 ** r15 |=> w7
+    | r10 =>
+      r8 |=> w0 ** r9 |=> w1 ** r11 |=> w3 **
+         r12 |=> w4 ** r13 |=> w5 ** r14 |=> w6 ** r15 |=> w7
+    | r11 =>
+      r8 |=> w0 ** r9 |=> w1 ** r10 |=> w2 **
+         r12 |=> w4 ** r13 |=> w5 ** r14 |=> w6 ** r15 |=> w7
+    | r12 =>
+      r8 |=> w0 ** r9 |=> w1 ** r10 |=> w2 **
+         r11 |=> w3 ** r13 |=> w5 ** r14 |=> w6 ** r15 |=> w7
+    | r13 =>
+      r8 |=> w0 ** r9 |=> w1 ** r10 |=> w2 **
+         r11 |=> w3 ** r12 |=> w4 ** r14 |=> w6 ** r15 |=> w7
+    | r14 =>
+      r8 |=> w0 ** r9 |=> w1 ** r10 |=> w2 **
+         r11 |=> w3 ** r12 |=> w4 ** r13 |=> w5 ** r15 |=> w7
+    | r15 =>
+      r8 |=> w0 ** r9 |=> w1 ** r10 |=> w2 **
+         r11 |=> w3 ** r12 |=> w4 ** r13 |=> w5 ** r14 |=> w6
+    | _ =>
+      r8 |=> w0 ** r9 |=> w1 ** r10 |=> w2 **
+         r11 |=> w3 ** r12 |=> w4 ** r13 |=> w5 ** r14 |=> w6 ** r15 |=> w7
+    end
+  end.
+
+Definition localRegs_rm_one (fm : Frame) (rr : GenReg) :=
+  match fm with
+  | consfm w0 w1 w2 w3 w4 w5 w6 w7 =>
+    match rr with
+    | r16 =>
+      r17 |=> w1 ** r18 |=> w2 ** r19 |=> w3 **
+         r20 |=> w4 ** r21 |=> w5 ** r22 |=> w6 ** r23 |=> w7
+    | r17 =>
+      r16 |=> w0 ** r18 |=> w2 ** r19 |=> w3 **
+         r20 |=> w4 ** r21 |=> w5 ** r22 |=> w6 ** r23 |=> w7
+    | r18 =>
+      r16 |=> w0 ** r17 |=> w1 ** r19 |=> w3 **
+         r20 |=> w4 ** r21 |=> w5 ** r22 |=> w6 ** r23 |=> w7
+    | r19 =>
+      r16 |=> w0 ** r17 |=> w1 ** r18 |=> w2 **
+         r20 |=> w4 ** r21 |=> w5 ** r22 |=> w6 ** r23 |=> w7
+    | r20 =>
+      r16 |=> w0 ** r17 |=> w1 ** r18 |=> w2 **
+         r19 |=> w3 ** r21 |=> w5 ** r22 |=> w6 ** r23 |=> w7
+    | r21 =>
+      r16 |=> w0 ** r17 |=> w1 ** r18 |=> w2 **
+         r19 |=> w3 ** r20 |=> w4 ** r22 |=> w6 ** r23 |=> w7
+    | r22 =>
+      r16 |=> w0 ** r17 |=> w1 ** r18 |=> w2 **
+          r19 |=> w3 ** r20 |=> w4 ** r21 |=> w5 ** r23 |=> w7
+    | r23 =>
+      r16 |=> w0 ** r17 |=> w1 ** r18 |=> w2 **
+          r19 |=> w3 ** r20 |=> w4 ** r21 |=> w5 ** r22 |=> w6
+    | _ =>
+      r16 |=> w0 ** r17 |=> w1 ** r18 |=> w2 ** r19 |=> w3 **
+         r20 |=> w4 ** r21 |=> w5 ** r22 |=> w6 ** r23 |=> w7
+    end
+  end.
+
+Definition inRegs_rm_one (fm : Frame) (rr : GenReg) :=
+  match fm with
+  | consfm w0 w1 w2 w3 w4 w5 w6 w7 =>
+    match rr with
+    | r24 =>
+      r25 |=> w1 ** r26 |=> w2 ** r27 |=> w3 **
+         r28 |=> w4 ** r29 |=> w5 ** r30 |=> w6 ** r31 |=> w7
+    | r25 =>
+      r24 |=> w0 ** r26 |=> w2 ** r27 |=> w3 **
+         r28 |=> w4 ** r29 |=> w5 ** r30 |=> w6 ** r31 |=> w7
+    | r26 =>
+      r24 |=> w0 ** r25 |=> w1 ** r26 |=> w2 **
+         r28 |=> w4 ** r29 |=> w5 ** r30 |=> w6 ** r31 |=> w7
+    | r27 =>
+      r24 |=> w0 ** r25 |=> w1 ** r26 |=> w2 **
+         r28 |=> w4 ** r29 |=> w5 ** r30 |=> w6 ** r31 |=> w7
+    | r28 =>
+      r24 |=> w0 ** r25 |=> w1 ** r26 |=> w2 **
+          r27 |=> w3 ** r29 |=> w5 ** r30 |=> w6 ** r31 |=> w7
+    | r29 =>
+      r24 |=> w0 ** r25 |=> w1 ** r26 |=> w2 **
+          r27 |=> w3 ** r28 |=> w4 ** r30 |=> w6 ** r31 |=> w7
+    | r30 =>
+      r24 |=> w0 ** r25 |=> w1 ** r26 |=> w2 **
+          r27 |=> w3 ** r28 |=> w4 ** r29 |=> w5 ** r31 |=> w7
+    | r31 =>
+      r24 |=> w0 ** r25 |=> w1 ** r26 |=> w2 **
+          r27 |=> w3 ** r28 |=> w4 ** r29 |=> w5 ** r30 |=> w6
+    | _ =>
+      r24 |=> w0 ** r25 |=> w1 ** r26 |=> w2 ** r27 |=> w3 **
+         r28 |=> w4 ** r29 |=> w5 ** r30 |=> w6 ** r31 |=> w7
+    end
+  end.
+
+Definition GenRegs_rm_one (greg_st : GenRegState) (rr : GenReg) :=
+  match greg_st with
+  | (fmg, fmo, fml, fmi) =>
+    globalRegs_rm_one fmg rr ** outRegs_rm_one fmo rr **
+                      localRegs_rm_one fml rr ** inRegs_rm_one fmi rr
+  end.
+
+Lemma GenRegs_split_one :
+  forall s grst p (rr : GenReg),
+    s |= GenRegs grst ** p ->
+    s |= rr |=> get_genreg_val grst rr ** GenRegs_rm_one grst rr ** p.
+Proof.
+  intros.
+  unfolds GenRegs.
+  destruct grst.
+  destruct p0.
+  destruct p0.
+  destruct f1, f2, f0, f.
+  destruct rr.
+  {
+    simpl get_genreg_val.
+    simpl GenRegs_rm_one.
+    unfold GlobalRegs, OutRegs, LocalRegs, InRegs in H.
+    >>>>>>>>>>>>>>>>>>>>
+  }
+  
+Theorem add_rule_reg :
+  forall grst rs rd p oexp v1 v2,
+    get_genreg_val grst rs = v1 -> eval_opexp_reg grst oexp = Some v2 ->
+    |- {{ GenRegs grst ** p }} add rs oexp rd
+                              {{ GenRegs (upd_genreg grst rd (v1 +ᵢ v2)) ** p }}.
+Proof.
+  intros.
+  eapply ins_conseq_rule.
+  eauto.
+  eapply add_rule; eauto.
+  {
+    intros.
+    simpl.
+    split.
+    {
+      instantiate (1 := v1).
+      sep_star_split_tac.
+      simpl in H5.
+      simpljoin1.
+      simpl.
+      eapply getR_eq_get_genreg_val in H1; eauto.
+      eapply get_R_merge_still; eauto.
+    }
+    {
+      instantiate (1 := v2).
+      sep_star_split_tac.
+      simpl in H5.
+      simpljoin1.
+      simpl.
+      eapply eval_opexp_merge_still; eauto.
+      eapply eval_opexp_reg_eq_eval_opexp; eauto.
+    }
+  }
+  {  
+    intros.
+    instantiate (2 := (get_genreg_val grst rd)).
+    instantiate (1 := (GenRegs_rm_one grst rd ** p)).
+  }
+  
+                         
